narrative.v
@@ -4,7 +4,6 @@ Import Utf8_core.
 Import ILLVarInt.MILL. (* only this *)
 Import ILLVarInt.M. (* this *)
 Import FormulaMultiSet. (* and this *)
-Import ILL_equiv.
 Require Import restrict2.
 
 Inductive narrative : Prop :=
@@ -14,57 +13,51 @@ Inductive narrative : Prop :=
 | Paral: narrative → narrative → narrative
 | Branch: narrative → narrative → narrative.
 
-
-Program Fixpoint ν Γ (φ:formula) (h: Γ ⊢ φ) {struct h}: narrative := 
-match h with
-  | Id _ _ p => Leaf
-  | Impl_R Γ p q x => ν _ _ x
-  | Impl_L Γ Δ Δ' p q r _ _ x x0 => Next (ν Δ p x) (Next (Impl(Implies p q)) (ν (q::Δ') r x0))
-  | Times_R Γ Δ Δ' p q heq x x0 =>  Paral (ν Δ p x) (ν Δ' q x0)
-  | Times_L Γ p q r _ x => ν _ _ x
-  | One_R _ _  => Leaf
-  | One_L Γ p _ x => ν _ _ x
-  | And_R Γ p q x x0 => Branch (ν _ _ x) (ν _ _ x0)
-  | And_L_1 Γ p q r _ x => ν _ _ x
-  | And_L_2 Γ p q r _ x => ν _ _ x
-  | Oplus_L Γ p q r _ x x0 => Branch (ν _ _ x) (ν _ _ x0)
-  | Oplus_R_1 Γ p q x => ν _ _ x
-  | Oplus_R_2 Γ p q x => ν _ _ x
-  | T_ Γ => Leaf
-  | Zero_ Γ p x => Leaf
-  | Bang_D Γ p q _ x => ν _ _ x
-  | Bang_C Γ p q _ x => ν _ _ x
-  | Bang_W Γ p q _ x => ν _ _ x
-end.
-
-Eval vm_compute in (ν _ _ originelle).
-
 Notation "∅" := Leaf.
 Notation "a ≻ b" := (Next a b) (at level 90, right associativity).
 Notation "a ⋈ b" := (Branch a b) (at level 91, right associativity).
 Notation "a ∣∣ b" := (Paral a b) (at level 92, right associativity).
 Notation "[ a ]" := (Impl a) (at level 89, right associativity).
 
-Eval vm_compute in (ν _ _ originelle).
+Show Obligation Tactic.
+Local Obligation Tactic :=
+  try solve [intuition; discriminate] ;  Tactics.program_simpl.
 
-Fixpoint reduc (x:narrative) : narrative:=
-  match x with
-    Leaf => Leaf
-    | Impl x1 => Impl x1
-    | Next x x0 => 
-      let x0' := reduc x0 in
-        match reduc x, reduc x0 with
-          | x',Leaf => x'
-          | Leaf, x0' => x0'
-          | x',x0' => Next x' x0'
-        end
-    | Paral x x0 => Paral (reduc x) (reduc x0)
-    | Branch x x0 => Branch (reduc x) (reduc x0)
+Definition simpl_narr b e p q :=
+  match b,e with
+    | ∅,∅ => [Implies p q]
+    | ∅,y=> [Implies p q] ≻ y
+    | x,∅ => x ≻ [Implies p q]
+    | x,y => x ≻ ([Implies p q] ≻ y)
   end.
 
-Eval vm_compute in (reduc (reduc (ν _ _ originelle))).
+Program Fixpoint ν Γ φ (h: Γ ⊢ φ) {struct h}: narrative := 
+match h with
+  | Id _ _ p => ∅
+  | Impl_R Γ p q x => ν _ _ x
+  | Impl_L Γ Δ Δ' p q r _ _ x x0 =>  simpl_narr (ν Δ p x) (ν (q::Δ') r x0) p q
+  | Times_R Γ Δ Δ' p q heq x x0 => (ν Δ p x) ∣∣ (ν Δ' q x0)
+  | Times_L Γ p q r _ x => ν _ _ x
+  | One_R _ _  => ∅
+  | One_L Γ p _ x => ν _ _ x
+  | And_R Γ p q x x0 => (ν _ _ x) ⋈ (ν _ _ x0)
+  | And_L_1 Γ p q r _ x => ν _ _ x
+  | And_L_2 Γ p q r _ x => ν _ _ x
+  | Oplus_L Γ p q r _ x x0 => (ν _ _ x) ⋈ (ν _ _ x0)
+  | Oplus_R_1 Γ p q x => ν _ _ x
+  | Oplus_R_2 Γ p q x => ν _ _ x
+  | T_ Γ => ∅
+  | Zero_ Γ p x => ∅
+  | Bang_D Γ p q _ x => ν _ _ x
+  | Bang_C Γ p q _ x => ν _ _ x
+  | Bang_W Γ p q _ x => ν _ _ x
+end.
+
+
+Eval vm_compute in (ν _ _ originelle).
 
 (* 
 [G ⊸ 1] ≻ ([R ⊸ E] ≻ [E ⊸ A] ⋈ [B ⊸ 1] ≻ [R ⊸ 1] ≻ [P ⊸ M])
 ⋈ [G ⊸ S] ≻ [R ⊸ 1] ≻ ([S ⊸ A] ⋈ [B ⊸ 1] ≻ [S ⊸ A])
  *)
+
